PivotBetree/PivotBetree.i.dfy
@@ -10,6 +10,7 @@ include "../Betree/Betree.i.dfy"
 include "../Betree/BetreeInv.i.dfy"
 include "../PivotBetree/PivotBetreeSpec.i.dfy"
 include "../MapSpec/UIStateMachine.s.dfy"
+include "PivotBetreeSpecRefinement.i.dfy"
 //
 // Like Betree, PivetBetree lowers the "lifted" op-sequences of PivotBetreeSpec
 // down to concrete state machine steps that advance the PivotBetreeBlockInterface
@@ -70,4 +71,286 @@ module PivotBetree refines UIStateMachine {
   predicate Next(k: Constants, s: Variables, s': Variables, uiop: UIOp) {
     exists step: Step :: NextStep(k, s, s', uiop, step)
   }
+
+  //////////////////////////////////////////////
+  ////// Invariants and refinement
+
+  //
+  // "Boilerplate" for the refinement/invariant proof for PivotBetree.
+  // Reasons about refinement between generic Ops.
+  // Relies on logic about specific ops from PivotBetreeSpecRefinement.
+  //
+  // This is "boilerplate" in that the difficult logic is about the Node and Op refinement
+  // in PivotBetreeSpecRefinement; this file just "lowers" that logic from ops down to
+  // concrete state machine steps.
+  //
+
+  import B = Betree
+  import BG = BetreeGraph
+  import PG = PivotBetreeGraph
+  import BBI = BetreeBlockInterface
+  import SpecRef = PivotBetreeSpecRefinement
+  import BInv = BetreeInv
+  import opened Sequences
+  import opened BucketWeights
+
+  function Ik(k: Constants) : B.Constants
+  {
+    B.Constants(BBI.Constants())
+  }
+
+  predicate ViewHasInvNodes(view: imap<Reference, Node>)
+  {
+    forall ref | ref in view :: InvNode(view[ref])
+  }
+
+  function IView(view: imap<Reference, Node>) : imap<Reference, BG.Node>
+  requires ViewHasInvNodes(view)
+  {
+    imap ref | ref in view :: SpecRef.INode(view[ref])
+  }
+  
+  function I(k: Constants, s: Variables) : B.Variables
+  requires ViewHasInvNodes(s.bcv.view)
+  {
+    B.Variables(BBI.Variables(IView(s.bcv.view)))
+  }
+
+  predicate Inv(k: Constants, s: Variables)
+  {
+    && ViewHasInvNodes(s.bcv.view)
+    && BInv.Inv(Ik(k), I(k, s))
+  }
+
+  lemma OpRefines(k: Constants, s: Variables, s': Variables, op: PG.Op)
+  requires InvNode(op.node)
+  requires ViewHasInvNodes(s.bcv.view)
+  requires BI.OpStep(k.bck, s.bcv, s'.bcv, op)
+  ensures ViewHasInvNodes(s'.bcv.view)
+  ensures BBI.OpStep(Ik(k).bck, I(k, s).bcv, I(k, s').bcv, SpecRef.IOp(op))
+  {
+    //BBI.OpStepPreservesInv(Ik(k).bck, I(k, s).bcv, I(k, s').bcv, SpecRef.IOp(op));
+  }
+
+  lemma IOpsAdditive(ops1: seq<PG.Op>, ops2: seq<PG.Op>)
+  requires forall i | 0 <= i < |ops1| :: InvNode(ops1[i].node)
+  requires forall i | 0 <= i < |ops2| :: InvNode(ops2[i].node)
+  ensures SpecRef.IOps(ops1 + ops2) == SpecRef.IOps(ops1) + SpecRef.IOps(ops2)
+  {
+    if (|ops2| == 0) {
+      assert ops2 == [];
+      assert SpecRef.IOps(ops2) == [];
+      assert ops1 + ops2 == ops1;
+      assert SpecRef.IOps(ops1 + ops2) == SpecRef.IOps(ops1) + SpecRef.IOps(ops2);
+    } else {
+      IOpsAdditive(ops1, ops2[..|ops2|-1]);
+      assert (ops1 + ops2)[..|ops1 + ops2|-1] == ops1 + ops2[..|ops2|-1];
+      assert SpecRef.IOps(ops1 + ops2)
+          == SpecRef.IOps((ops1 + ops2)[..|ops1 + ops2|-1]) + [SpecRef.IOp((ops1 + ops2)[|ops1 + ops2| - 1])]
+          == SpecRef.IOps(ops1 + ops2[..|ops2|-1]) + [SpecRef.IOp((ops1 + ops2)[|ops1 + ops2| - 1])]
+          == SpecRef.IOps(ops1) + SpecRef.IOps(ops2[..|ops2|-1]) + [SpecRef.IOp((ops1 + ops2)[|ops1 + ops2| - 1])]
+          == SpecRef.IOps(ops1) + SpecRef.IOps(ops2[..|ops2|-1]) + [SpecRef.IOp(ops2[|ops2| - 1])]
+          == SpecRef.IOps(ops1) + SpecRef.IOps(ops2);
+    }
+  }
+
+  lemma TransactionRefines(k: Constants, s: Variables, s': Variables, ops: seq<PG.Op>)
+  requires forall i | 0 <= i < |ops| :: InvNode(ops[i].node)
+  requires ViewHasInvNodes(s.bcv.view)
+  requires BI.Transaction(k.bck, s.bcv, s'.bcv, ops)
+  ensures ViewHasInvNodes(s'.bcv.view)
+  ensures BBI.Transaction(Ik(k).bck, I(k, s).bcv, I(k, s').bcv, SpecRef.IOps(ops))
+  decreases |ops|
+  {
+    if (|ops| == 0) {
+    } else if (|ops| == 1) {
+      OpRefines(k, s, s', ops[0]);
+    } else {
+      var ops1, mid, ops2 := BI.SplitTransaction(k.bck, s.bcv, s'.bcv, ops);
+      var smid := Variables(mid);
+
+      forall i | 0 <= i < |ops1| ensures InvNode(ops1[i].node)
+      {
+        assert ops1[i].node == ops[i].node;
+      }
+      forall i | 0 <= i < |ops2| ensures InvNode(ops2[i].node)
+      {
+        assert ops2[i].node == ops[i + |ops1|].node;
+      }
+
+      TransactionRefines(k, s, smid, ops1);
+      TransactionRefines(k, smid, s', ops2);
+      BBI.JoinTransactions(Ik(k).bck, I(k, s).bcv, I(k, smid).bcv, I(k, s').bcv, SpecRef.IOps(ops1), SpecRef.IOps(ops2));
+      IOpsAdditive(ops1, ops2);
+      //assert SpecRef.IOps(ops) == SpecRef.IOps(ops1) + SpecRef.IOps(ops2); // TODO
+    }
+  }
+
+  lemma ReadsRefines(k: Constants, s: Variables, ops: seq<PG.ReadOp>)
+  requires forall i | 0 <= i < |ops| :: InvNode(ops[i].node)
+  requires forall i | 0 <= i < |ops| :: WFNode(ops[i].node)
+  requires ViewHasInvNodes(s.bcv.view)
+  requires BI.Reads(k.bck, s.bcv, ops)
+  ensures BBI.Reads(Ik(k).bck, I(k, s).bcv, SpecRef.IReadOps(ops))
+  decreases |ops|
+  {
+    if (|ops| == 0) {
+    } else {
+      ReadsRefines(k, s, DropLast(ops));
+      forall op' | op' in SpecRef.IReadOps(ops)
+      ensures BBI.ReadStep(Ik(k).bck, I(k, s).bcv, op')
+      {
+        var i :| 0 <= i < |SpecRef.IReadOps(ops)| && SpecRef.IReadOps(ops)[i] == op';
+        if (i == |ops| - 1) {
+          var op := ops[i];
+          //assert op' == SpecRef.IReadOp(op);
+          assert BI.ReadStep(k.bck, s.bcv, op);
+          /*
+          assert op.ref in s.bcv.view;
+          assert op'.ref == op.ref;
+          assert op'.ref in s.bcv.view;
+          assert op'.ref in I(k, s).bcv.view;
+          assert I(k, s).bcv.view[op'.ref]
+              == SpecRef.INode(s.bcv.view[op.ref])
+              == op'.node;
+          assert BBI.ReadStep(Ik(k).bck, I(k, s).bcv, op');
+          */
+        } else {
+          //assert BBI.ReadStep(Ik(k).bck, I(k, s).bcv, SpecRef.IReadOps(ops)[i]);
+        }
+      }
+    }
+  }
+
+  /*lemma ReadOpsBucketsWellMarshalledOfValidStep(k: Constants, s: Variables, betreeStep: BetreeStep)
+  requires ValidBetreeStep(betreeStep)
+  requires BI.Reads(k.bck, s.bcv, BetreeStepReads(betreeStep))
+  ensures SpecRef.ReadOpsBucketsWellMarshalled(BetreeStepReads(betreeStep))
+  {
+    var readOps := BetreeStepReads(betreeStep);
+    forall i, j |
+      0 <= i < |readOps| &&
+      0 <= j < |readOps[i].node.buckets|
+    ensures BucketWellMarshalled(readOps[i].node.buckets[j])
+    {
+      assert BI.ReadStep(k.bck, s.bcv, readOps[i]);
+      assert readOps[i].node == s.bcv.view[readOps[i].ref];
+    }
+  }*/
+
+  lemma BetreeStepRefines(k: Constants, s: Variables, s': Variables, uiop: UIOp, betreeStep: BetreeStep)
+  requires Inv(k, s)
+  requires NextStep(k, s, s', uiop, BetreeStep(betreeStep))
+  ensures Inv(k, s')
+  //ensures B.NextStep(Ik(k), I(k,s), I(k,s'), uiop, B.BetreeStep(SpecRef.IStep(betreeStep)))
+  ensures B.Next(Ik(k), I(k,s), I(k,s'), uiop)
+  {
+    if (betreeStep.BetreeRepivot?) {
+      SpecRef.RepivotPreservesNode(betreeStep.repivot);
+
+      assert B.NextStep(Ik(k), I(k,s), I(k,s'), uiop, B.StutterStep);
+      BInv.NextPreservesInv(Ik(k), I(k, s), I(k, s'), uiop);
+    } else {
+      forall i | 0 <= i < |BetreeStepReads(betreeStep)|
+      ensures InvNode(BetreeStepReads(betreeStep)[i].node)
+      {
+        assert BI.ReadStep(k.bck, s.bcv, BetreeStepReads(betreeStep)[i]);
+        assert s.bcv.view[BetreeStepReads(betreeStep)[i].ref]
+            == BetreeStepReads(betreeStep)[i].node;
+      }
+
+      SpecRef.RefinesValidBetreeStep(betreeStep);
+      SpecRef.RefinesReadOps(betreeStep);
+      SpecRef.RefinesOps(betreeStep);
+      TransactionRefines(k, s, s', BetreeStepOps(betreeStep));
+      ReadsRefines(k, s, BetreeStepReads(betreeStep));
+
+      /*
+      match betreeStep {
+        case BetreeQuery(q) => {
+          assert B.Betree(Ik(k), I(k,s), I(k,s'), uiop, SpecRef.IStep(betreeStep));
+          assert B.NextStep(Ik(k), I(k,s), I(k,s'), uiop, B.BetreeStep(SpecRef.IStep(betreeStep)));
+        }
+        case BetreeInsert(ins) => 
+        assert B.NextStep(Ik(k), I(k,s), I(k,s'), uiop, B.BetreeStep(SpecRef.IStep(betreeStep)));
+        case BetreeFlush(flush) => 
+        assert B.NextStep(Ik(k), I(k,s), I(k,s'), uiop, B.BetreeStep(SpecRef.IStep(betreeStep)));
+        case BetreeGrow(growth) => 
+        assert B.NextStep(Ik(k), I(k,s), I(k,s'), uiop, B.BetreeStep(SpecRef.IStep(betreeStep)));
+        case BetreeSplit(fusion) => 
+        assert B.NextStep(Ik(k), I(k,s), I(k,s'), uiop, B.BetreeStep(SpecRef.IStep(betreeStep)));
+        case BetreeMerge(fusion) => 
+        assert B.NextStep(Ik(k), I(k,s), I(k,s'), uiop, B.BetreeStep(SpecRef.IStep(betreeStep)));
+      }
+      */
+      assert B.NextStep(Ik(k), I(k,s), I(k,s'), uiop, B.BetreeStep(SpecRef.IStep(betreeStep)));
+      BInv.NextPreservesInv(Ik(k), I(k, s), I(k, s'), uiop);
+    }
+  }
+
+  lemma GCStepRefines(k: Constants, s: Variables, s': Variables, uiop: UIOp, refs: iset<Reference>)
+  requires Inv(k, s)
+  requires NextStep(k, s, s', uiop, GCStep(refs))
+  ensures Inv(k, s')
+  ensures B.NextStep(Ik(k), I(k,s), I(k,s'), uiop, B.GCStep(refs))
+  {
+    assert B.NextStep(Ik(k), I(k,s), I(k,s'), uiop, B.GCStep(refs));
+    BInv.NextPreservesInv(Ik(k), I(k, s), I(k, s'), uiop);
+  }
+
+  lemma StutterStepRefines(k: Constants, s: Variables, s': Variables, uiop: UIOp)
+  requires Inv(k, s)
+  requires NextStep(k, s, s', uiop, StutterStep)
+  ensures Inv(k, s')
+  ensures B.NextStep(Ik(k), I(k,s), I(k,s'), uiop, B.StutterStep)
+  {
+  }
+
+  lemma PivotBetreeRefinesBetreeNextStep(k: Constants, s: Variables, s': Variables, uiop: UIOp, step: Step)
+    requires Inv(k, s)
+    requires NextStep(k, s, s', uiop, step)
+    ensures Inv(k, s')
+    ensures B.Next(Ik(k), I(k, s), I(k, s'), uiop)
+  {
+    match step {
+      case BetreeStep(betreeStep) => BetreeStepRefines(k, s, s', uiop, betreeStep);
+      case GCStep(refs) => GCStepRefines(k, s, s', uiop, refs);
+      case StutterStep => StutterStepRefines(k, s, s', uiop);
+    }
+  }
+
+  lemma InitImpliesInv(k: Constants, s: Variables)
+  // declared in UIStateMachine
+  {
+    RefinesInit(k, s);
+  }
+
+  lemma NextPreservesInv(k: Constants, s: Variables, s': Variables, uiop: UIOp)
+  // declared in UIStateMachine
+  {
+    var step :| NextStep(k, s, s', uiop, step);
+    PivotBetreeRefinesBetreeNextStep(k, s, s', uiop, step);
+  }
+
+  lemma RefinesInit(k: Constants, s: Variables)
+    requires Init(k, s)
+    ensures Inv(k, s)
+    ensures B.Init(Ik(k), I(k, s))
+  {
+    reveal_WeightBucketList();
+    reveal_WeightBucket();
+    assert SpecRef.INode(EmptyNode()) == B.EmptyNode();
+    BInv.InitImpliesInv(Ik(k), I(k, s));
+  }
+
+  lemma RefinesNext(k: Constants, s: Variables, s': Variables, uiop: UIOp)
+    requires Inv(k, s)
+    requires Next(k, s, s', uiop)
+    ensures Inv(k, s')
+    ensures B.Next(Ik(k), I(k, s), I(k, s'), uiop)
+  {
+    var step :| NextStep(k, s, s', uiop, step);
+    PivotBetreeRefinesBetreeNextStep(k, s, s', uiop, step);
+  }
+
 }
