MapSpec/UIStateMachine.s.dfy
@@ -8,4 +8,15 @@ abstract module UIStateMachine {
   type Variables(!new)
   predicate Init(k: Constants, s: Variables)
   predicate Next(k: Constants, s: Variables, s': Variables, uiop: UIOp)
+
+  predicate Inv(k: Constants, s: Variables)
+
+  lemma InitImpliesInv(k: Constants, s: Variables)
+  requires Init(k, s)
+  ensures Inv(k, s)
+
+  lemma NextPreservesInv(k: Constants, s: Variables, s': Variables, uiop: UIOp)
+  requires Inv(k, s)
+  requires Next(k, s, s', uiop)
+  ensures Inv(k, s')
 }
